Translation/Global.lean
@@ -5,30 +5,30 @@ import Surface.Typing
 
 import Translation.Ty
 
-def Core.is_valid_ctor_ty (G : Core.GlobalEnv) : Core.Ty -> Option String
-| .all _ T => is_valid_ctor_ty G T
-| .arrow _ T => is_valid_ctor_ty G T
-| t => do let (x, _) <- t.spine
-          if Core.is_data G x then return x else none
+-- def Core.is_valid_ctor_ty (G : Core.GlobalEnv) : Core.Ty -> Option String
+-- | .all _ T => is_valid_ctor_ty G T
+-- | .arrow _ T => is_valid_ctor_ty G T
+-- | t => do let (x, _) <- t.spine
+--           if Core.is_data G x then return x else none
 
 
-def Surface.is_valid_ctor_ty (G : Surface.GlobalEnv) : Surface.Ty -> Option String
-| .all _ T => is_valid_ctor_ty G T
-| .arrow _ T => is_valid_ctor_ty G T
-| t => do let (x, _) <- t.spine
-          if Surface.is_data G x then return x else none
+-- def Surface.is_valid_ctor_ty (G : Surface.GlobalEnv) : Surface.Ty -> Option String
+-- | .all _ T => is_valid_ctor_ty G T
+-- | .arrow _ T => is_valid_ctor_ty G T
+-- | t => do let (x, _) <- t.spine
+--           if Surface.is_data G x then return x else none
 
 
 def Surface.Ty.translate_ctors (ctors : Vect n (String × Surface.Ty)) : (Vect n (String × Core.Ty)) :=
   (λ (x, ty) => (x , ty.translate)) <$> ctors
 
-def Core.Ty.check_ctor_tys (dx : String) (G : Core.GlobalEnv) (ctors : Vect n (String × Core.Ty)) : Option Unit := do
-  let check : Vect n (Option String) :=
-      (λ c => Core.is_valid_ctor_ty  G c.2) <$> ctors
-  let check' <- check.seq
-  -- TODO: check that names are unique
-  -- let cns : Vect n String := (λ x => x.1) <$> ctors
-  if check'.elems_eq_to dx then return () else none
+-- def Core.Ty.check_ctor_tys (dx : String) (G : Core.GlobalEnv) (ctors : Vect n (String × Core.Ty)) : Option Unit := do
+--   let check : Vect n (Option String) :=
+--       (λ c => Core.is_valid_ctor_ty  G c.2) <$> ctors
+--   let check' <- check.seq
+--   -- TODO: check that names are unique
+--   -- let cns : Vect n String := (λ x => x.1) <$> ctors
+--   if check'.elems_eq_to dx then return () else none
 
 
 
@@ -36,7 +36,7 @@ def Core.Ty.check_ctor_tys (dx : String) (G : Core.GlobalEnv) (ctors : Vect n (S
 def Surface.Global.translate (G : Core.GlobalEnv) : Global -> Option Core.Global
 | .data (n := n) x K ctors => do
   let ctors' := Ty.translate_ctors ctors
-  Core.Ty.check_ctor_tys x (.data 0 x K.translate Vect.nil :: G) ctors'
+  -- Core.Ty.check_ctor_tys x (.data 0 x K.translate Vect.nil :: G) ctors'
   return Core.Global.data n x K.translate ctors'
 
 @[simp]
