Translation/Global/Lemmas.lean
@@ -14,37 +14,35 @@ theorem Translation.Global.is_data_sound x :
   Surface.is_data G x ->
   Core.is_data G' x := by sorry
 
-theorem Translation.Ty.valid_ctor_ty_sound {G : Core.GlobalEnv} :
-  Core.is_valid_ctor_ty G T == some x -> Core.ValidCtor G x T := by
-intro h
-fun_induction Core.is_valid_ctor_ty <;> simp at *
-case _ ih => replace ih := ih h; apply Core.ValidCtor.all ih
-case _ ih => replace ih := ih h; apply Core.ValidCtor.arrow ih
-case _ =>
-  rw[Option.bind_eq_some_iff] at h; rcases h with ⟨tnf, h1, h2⟩;
-  simp at h2; rcases h2 with ⟨h2, e⟩; subst x
-  apply Core.ValidCtor.base; apply h1; apply h2
+-- theorem Translation.Ty.valid_ctor_ty_sound {G : Core.GlobalEnv} :
+--   Core.is_valid_ctor_ty G T == some x -> Core.ValidCtor G x T := by
+-- intro h
+-- fun_induction Core.is_valid_ctor_ty <;> simp at *
+-- case _ ih => replace ih := ih h; apply Core.ValidCtor.all ih
+-- case _ ih => replace ih := ih h; apply Core.ValidCtor.arrow ih
+-- case _ =>
+--   rw[Option.bind_eq_some_iff] at h; rcases h with ⟨tnf, h1, h2⟩;
+--   simp at h2; rcases h2 with ⟨h2, e⟩; subst x
+--   apply Core.ValidCtor.base; apply h1; apply h2
 
-theorem Translation.Ty.valid_ctor_ty_sound' {G : Surface.GlobalEnv} :
-  Surface.is_valid_ctor_ty G T == some x -> Surface.ValidCtor G x T := by
-intro h
-fun_induction Surface.is_valid_ctor_ty <;> simp at *
-case _ ih => replace ih := ih h; apply Surface.ValidCtor.all ih
-case _ ih => replace ih := ih h; apply Surface.ValidCtor.arrow ih
-case _ =>
-  rw[Option.bind_eq_some_iff] at h; rcases h with ⟨tnf, h1, h2⟩;
-  simp at h2; rcases h2 with ⟨h2, e⟩; subst x
-  apply Surface.ValidCtor.base; apply h1; apply h2
+-- theorem Translation.Ty.valid_ctor_ty_sound' {G : Surface.GlobalEnv} :
+--   Surface.is_valid_ctor_ty G T == some x -> Surface.ValidCtor G x T := by
+-- intro h
+-- fun_induction Surface.is_valid_ctor_ty <;> simp at *
+-- case _ ih => replace ih := ih h; apply Surface.ValidCtor.all ih
+-- case _ ih => replace ih := ih h; apply Surface.ValidCtor.arrow ih
+-- case _ =>
+--   rw[Option.bind_eq_some_iff] at h; rcases h with ⟨tnf, h1, h2⟩;
+--   simp at h2; rcases h2 with ⟨h2, e⟩; subst x
+--   apply Surface.ValidCtor.base; apply h1; apply h2
 
 theorem Translation.Ty.ValidCtor :
-  ⊢s G ->
-  G.translate = some G' ->
-  Surface.ValidCtor G x T -> Core.ValidCtor G' x ⟦T⟧ := by
-intro wf gt h; induction h <;> simp at *
+  Surface.ValidCtor x T -> Core.ValidCtor x ⟦T⟧ := by
+intro h; induction h <;> simp at *
 case base h1 h2 =>
-  replace lem := Translation.Ty.Spine h1 rfl
+  replace lem := Translation.Ty.Spine h2 rfl
   rcases lem with ⟨_, lem⟩
-  constructor; assumption; apply Translation.Global.is_data_sound x wf gt h2
+  constructor; assumption
 case all ih => apply Core.ValidCtor.all ih
 case arrow ih => apply Core.ValidCtor.arrow ih
 
@@ -67,17 +65,17 @@ theorem Surface.GlobalEnvWf.empty_data_wkn x K :
  · assumption
 
 
-theorem Translation.Ty.check_valid_ctors_sound ctors :
-  (∀ (i : Fin n) (y : String) (T : Surface.Ty),
-    ctors i = (y, T) →
-      (Surface.Global.data x K Vect.nil :: G)&[] ⊢s T : Surface.Kind.base b`★ ∧
-        Surface.ValidCtor (Surface.Global.data x K Vect.nil :: G) x T ∧ x ≠ y ∧ Surface.lookup y G = none) ->
-  Core.Ty.check_ctor_tys x (Core.Global.data 0 x ⟦K⟧ Vect.nil :: G') (Surface.Ty.translate_ctors ctors) = some ()
-:= by
-intro h
-unfold Core.Ty.check_ctor_tys
-simp;
-sorry
+-- theorem Translation.Ty.check_valid_ctors_sound ctors :
+--   (∀ (i : Fin n) (y : String) (T : Surface.Ty),
+--     ctors i = (y, T) →
+--       (Surface.Global.data x K Vect.nil :: G)&[] ⊢s T : Surface.Kind.base b`★ ∧
+--         Surface.ValidCtor x T ∧ x ≠ y ∧ Surface.lookup y G = none) ->
+--   Core.Ty.check_ctor_tys x (Core.Global.data 0 x ⟦K⟧ Vect.nil :: G') (Surface.Ty.translate_ctors ctors) = some ()
+-- := by
+-- intro h
+-- unfold Core.Ty.check_ctor_tys
+-- simp;
+-- sorry
 
 
 
@@ -94,73 +92,23 @@ intro wf h1 h2 h3 wfc; induction g <;> simp at *
 cases h1
 case _ n x K ctors cns lk cnsdef ctor_trans =>
 let ctors' : Vect n (String × Core.Ty) := Surface.Ty.translate_ctors ctors
-exists Core.Global.data n x ⟦K⟧ ctors'
-rw[Option.bind_eq_some_iff];
-apply And.intro
-· exists ()
+apply Core.GlobalWf.data
+· intro i y T e;
+  replace ctor_trans := ctor_trans i (ctors i).fst (ctors i).snd rfl;
+  rcases ctor_trans with ⟨k1, k2, k3, k4⟩
+  rcases e with ⟨e1, e2⟩;
+  have lemG := Translation.Global.empty_data_wkn x K h2
+  have wfG := Surface.GlobalEnvWf.empty_data_wkn x K wf lk
+  have lem := Translation.Ty.sound wfG (G := .data x K Vect.nil :: G) ⟨k1,lemG, rfl⟩
   apply And.intro
-  · sorry
-  · simp; unfold ctors'; simp;
-. apply Core.GlobalWf.data
-  · intro i y T e;
-    replace ctor_trans := ctor_trans i (ctors i).fst (ctors i).snd rfl;
-    rcases ctor_trans with ⟨k1, k2, k3, k4⟩
-    simp [ctors'] at e; rcases e with ⟨e1, e2⟩;
-    have lemG := Translation.Global.empty_data_wkn x K h2
-    have wfG := Surface.GlobalEnvWf.empty_data_wkn x K wf lk
-    have lem := Translation.Ty.sound wfG (G := .data x K Vect.nil :: G) ⟨k1,lemG, rfl⟩
-    apply And.intro
-    · rcases lem with ⟨K', T', e1, e2, e3⟩;
-      simp at e1; subst e1; subst e2; simp [Surface.KindEnv.translate] at e3; apply e3
-    · apply And.intro
-      · apply Translation.Ty.ValidCtor wfG lemG k2
-      · apply And.intro; assumption
-        apply h3; apply k4
-  · assumption
-  · apply h3 _ lk
-
-  -- exists ctors';
---   apply And.intro
---   · simp [Surface.Ty.translate_ctors]
-
---     unfold Vect.seq;
---     generalize zdef : Vect.seq_lemma (fun n =>
---         (Core.is_valid_ctor_ty (Core.Global.data 0 x ⟦K⟧ Vect.nil :: G') ⟦(ctors n).snd⟧).bind fun __discr =>
---           some ((ctors n).fst, ⟦(ctors n).snd⟧)) = z at *
---     cases z <;> simp at *
---     case inr v => funext; case _ i =>   unfold ctors'; simp
---     case inl v =>
---       rcases v with ⟨j, v⟩
---       have lem := Option.not_isSome_iff_eq_none.1 v
---       replace lem := Option.bind_eq_none'.1 lem ((ctors j).fst , ⟦(ctors j).snd⟧) x
---       replace ctor_trans := ctor_trans j (ctors j).fst (ctors j).snd rfl
---       rcases ctor_trans with ⟨k1, k2, k3, k4⟩
---       have lemG := Translation.Global.empty_data_wkn x K h2
---       have wfG := Surface.GlobalEnvWf.empty_data_wkn x K wf lk
---       have k2' := Translation.Ty.ValidCtor wfG lemG k2
---       -- have k2' := Translation.Ty.ValidCtor k2
-
---       sorry
-
---   · simp
--- · apply Core.GlobalWf.data
---   · intro i y T e;
---     replace ctor_trans := ctor_trans i (ctors i).fst (ctors i).snd rfl;
---     rcases ctor_trans with ⟨k1, k2, k3, k4⟩
---     simp [ctors'] at e; rcases e with ⟨e1, e2⟩; subst y; subst T
---     have lemG := Translation.Global.empty_data_wkn x K h2
---     have wfG := Surface.GlobalEnvWf.empty_data_wkn x K wf lk
---     have lem := Translation.Ty.sound wfG (G := .data x K Vect.nil :: G) ⟨k1,lemG, rfl⟩
---     apply And.intro
---     · rcases lem with ⟨K', T', e1, e2, e3⟩;
---       simp at e1; subst e1; subst e2; simp [Surface.KindEnv.translate] at e3; apply e3
---     · apply And.intro
---       · apply Translation.Ty.ValidCtor wfG lemG k2
---       · apply And.intro; assumption
---         apply h3; apply k4
---   · assumption
---   · apply h3 _ lk
-
+  · rcases lem with ⟨K', T', e1, e2, e3⟩;
+    simp at e1; subst e1; subst e2; simp [Surface.KindEnv.translate] at e3; apply e3
+  · apply And.intro
+    · apply Translation.Ty.ValidCtor k2
+    · apply And.intro; assumption
+      apply h3; apply k4
+· assumption
+· apply h3 _ lk
 
 theorem Translation.ListGlobalWf.sound_isSome :
   ⊢s G ->
